Primitive_Matchers/IPPortSpace_Syntax.thy
@@ -1,30 +1,30 @@
 theory IPPortSpace_Syntax
-imports Main String "../Bitmagic/IPv4Addr" "../Bitmagic/BitrangeLists" IPSpace_Syntax
+imports Main String "../Bitmagic/IPv4Addr" "../Bitmagic/BitrangeLists" IPSpace_Syntax Protocol Iface Simple_Packet
 begin
+
+(*TODO: unify protocol types*)
+hide_type(open) ipt_protocol
+hide_const(open) ProtAll ProtTCP ProtUDP
 
 section{*Primitive Matchers: IP Space and Layer 4 Ports Matcher*}
 
 text{*Primitive Match Conditions which only support IPv4 addresses,  layer 4 protocols, and layer 4 ports.
 *}
 
-datatype ipt_protocol = ProtAll | ProtTCP | ProtUDP
-
 (*list of (start, end) port ranges*)
 type_synonym ipt_ports = "(16 word \<times> 16 word) list"
 
-datatype ipport_rule_match = Src ipt_ipv4range | Dst ipt_ipv4range | Prot ipt_protocol | Src_Ports ipt_ports | Dst_Ports ipt_ports | Extra string
+
+text{*I lied. It will not only be an Ip+Port matcher but an Ip+Port+Iface matcher*}
+datatype ipport_rule_match = Src ipt_ipv4range | Dst ipt_ipv4range | IIface iface | OIface iface | Prot protocol | Src_Ports ipt_ports | Dst_Ports ipt_ports | Extra string
 
 
 
-subsection{*Example Packet*}
-  record packet_with_ports = packet +
-        src_port :: "16 word"
-        dst_port :: "16 word"
+(*subsection{*Example Packet*}*)
+ (*TODO: unify: packet + *)
 
-  value "\<lparr>src_ip = ipv4addr_of_dotteddecimal (192,168,2,45), dst_ip= ipv4addr_of_dotteddecimal (173,194,112,111),
-         prot=protPacket.ProtTCP, src_port=2065, dst_port=80\<rparr>"
-
-
+  value "\<lparr>p_iiface = ''eth0'', p_oiface = ''eth1'', p_src = ipv4addr_of_dotteddecimal (192,168,2,45), p_dst= ipv4addr_of_dotteddecimal (173,194,112,111),
+         p_proto=TCP, p_sport=2065, p_dport=80\<rparr>"
 
 
 fun ports_to_set :: "ipt_ports \<Rightarrow> (16 word) set" where
