Primitive_Matchers/Simple_Packet.thy
@@ -1,0 +1,15 @@
+theory Simple_Packet
+imports "../Bitmagic/IPv4Addr" Protocol
+begin
+
+section{*Simple Packet*}
+  text{*Packet constants are prefixed with p_*}
+  record simple_packet = p_iiface :: string
+                         p_oiface :: string
+                         p_src :: ipv4addr
+                         p_dst :: ipv4addr
+                         p_proto :: primitive_protocol
+                         p_sport :: "16 word"
+                         p_dport :: "16 word"
+
+end
